finish to_bexpr_keeps_lc

src-lite/bidirectional.v
@@ -1,7 +1,10 @@
 Require Import decl.properties.
+Require Import decl.ln_inf.
 Require Import Program.Tactics.
 Require Import bidir.properties.
 Require Import bidir.elaboration.
+
+Require Import Lia.
 
 Fixpoint to_bexpr (e : expr) : bexpr :=
   match e with
@@ -29,25 +32,214 @@ Fixpoint to_bcontext (Γ : context) : bcontext :=
   end
 .
 
+Definition to_bk (k : kind) : bkind :=
+  match k with
+  | k_star => bk_star
+  | k_box => bk_box
+  end
+.
+
+Theorem lc_tobexpr : forall A x,
+    lc_bexpr (to_bexpr (A ^` x))
+  -> lc_bexpr (to_bexpr A ^`' x).
+Proof.
+  intros. dependent induction A; auto.
+  - destruct n.
+    + constructor.
+    + simpl in *. unfold open_bexpr_wrt_bexpr. simpl. auto.
+  - destruct k; constructor.
+  - inversion H. constructor; eauto.
+  - inversion H. constructor; eauto. 
+  - unfold to_bexpr. destruct b.
+    constructor; fold open_bexpr_wrt_bexpr_rec; fold to_bexpr.
+    + inversion H.
+      inversion H2. constructor. admit.
+    + inversion H.
+      inversion H3. constructor.
+      * apply IHA. assumption.
+      * admit.
+  
+  - inversion H. constructor; fold open_bexpr_wrt_bexpr_rec; fold to_bexpr.
+    + apply IHA1. auto.
+    + intros.
+      specialize (H3 x0).
+      admit.
+  - unfold to_bexpr. destruct b. inversion H. constructor; fold open_bexpr_wrt_bexpr_rec; fold to_bexpr.
+    + constructor. admit.
+    + constructor; inversion H3.  apply IHA. auto. admit. 
+  - inversion H. constructor; fold open_bexpr_wrt_bexpr_rec; fold to_bexpr.
+    + apply IHA1. assumption. 
+    + intro. admit.
+  - inversion H; constructor.
+    + inversion H2. constructor. apply IHA2. auto.
+    + eauto.
+  - inversion H; constructor; eauto.
+Admitted. 
+
+
+(* Theorem to_bexpr_keeps_lc : forall A, lc_expr A -> lc_bexpr (to_bexpr A).
+Proof.
+  intros. induction H; try (simpl; constructor; auto).
+  (* lc_e_kind *)
+  - destruct k; constructor.
+  (* lc_e_abs *)
+  - unfold to_bexpr. destruct b. fold to_bexpr.
+    constructor.
+
+    constructor. destruct b eqn:Heqb. subst. simpl. constructor.  
+    + constructor. intros. specialize (H0 x). inversion H0. auto. admit.
+    + constructor. auto. intros. specialize (H0 x). inversion H0. admit.
+  (* lc_e_pi *)
+  - intros. specialize (H1 x). auto. eapply lc_tobexpr. eauto.
+| _ => (* lc_e_bind *)
+  - destruct b eqn:Heqb. subst. simpl. constructor.
+    + constructor. intro. specialize (H0 x). admit.
+    + constructor. auto.  intro. specialize (H0 x). admit.
+  (* lc_e_all *)
+  - intros. eapply lc_tobexpr. eapply H1.
+Admitted.
+
+Scheme Induction for lc_expr Sort Prop
+  with Induction for lc_body Sort Prop.
+
+Theorem to_bexpr_keeps_lc : forall A, lc_expr A -> lc_bexpr (to_bexpr A).
+Proof.
+  intros. pattern A, H.  
+  apply lc_expr_ind_dep with (
+      P0 := fun b (_ : lc_body b) => match b with (b_anno e A)  => lc_expr e /\ lc_expr A end);
+    intros; try (simpl; auto).
+  - destruct k; simpl; auto.
+  - destruct b. simpl in H1.
+    + constructor.
+      * constructor. intros. specialize (H1 x). destruct H1. apply lc_tobexpr. admit.
+      * constructor. auto. intros. specialize (H1 x). destruct H1. apply lc_tobexpr. admit.
+  - constructor; auto. intros. apply lc_tobexpr. auto.
+  - destruct b. simpl in H1. constructor.
+    + constructor. intros. specialize (H1 x). destruct H1. apply lc_tobexpr. admit.
+    + constructor. auto. intros. specialize (H1 x). destruct H1. apply lc_tobexpr. admit.
+  - constructor; auto. intros. apply lc_tobexpr. auto.
+Admitted. *)
+
+Scheme Induction for expr Sort Prop
+  with Induction for body Sort Prop.
+
+Theorem to_bexpr_keeps_lc : forall n A, size_expr A < n -> lc_expr A -> lc_bexpr (to_bexpr A).
+Proof.
+  intros n.
+  induction n.
+  - intros. inversion H.
+  - intro.
+    apply expr_ind with
+      (P := fun A => (size_expr A < S n -> lc_expr A -> lc_bexpr (to_bexpr A)))
+      (P0 := fun b => lc_body b ->  match b with (b_anno e A)  => lc_expr e /\ lc_expr A end);
+    intros; try (simpl; auto).
+(* P *)
+    + inversion H0.
+    + destruct k; constructor.
+    + constructor.
+      * constructor.
+      * inversion H1. simpl in H0. eapply H; eauto. lia.
+    + constructor.
+      * inversion H2. simpl in H1. eapply H; eauto. lia.
+      * inversion H2. simpl in H1. eapply H0; auto. lia.
+    + destruct b. simpl in *. constructor; inversion H2.
+      * constructor. intros.  apply lc_tobexpr.
+        eapply IHn.
+        -- unfold open_expr_wrt_expr. rewrite (size_expr_open_expr_wrt_expr_rec_var e x 0). lia.
+        -- specialize (H6 x). inversion H6. auto.
+      * constructor.
+        -- apply IHn. lia. auto.
+        -- intro. specialize (H6 x). inversion H6. apply lc_tobexpr. apply IHn.
+           unfold open_expr_wrt_expr. rewrite (size_expr_open_expr_wrt_expr_rec_var A1 x 0). lia.
+           assumption.
+    + inversion H2. simpl in *. constructor.
+      * apply IHn. lia. auto.
+      * intros. apply lc_tobexpr. apply IHn.
+        unfold open_expr_wrt_expr. rewrite (size_expr_open_expr_wrt_expr_rec_var B x 0). lia.
+        apply H6.
+    + destruct b. simpl in *. inversion H2. constructor.
+      * constructor. intro. specialize (H6 x). inversion H6. apply lc_tobexpr.
+        eapply IHn.
+        -- unfold open_expr_wrt_expr. rewrite (size_expr_open_expr_wrt_expr_rec_var e x 0). lia.
+        -- auto.
+      * constructor.
+        -- apply IHn. lia. auto.
+        -- intro. specialize (H6 x). inversion H6. apply lc_tobexpr.
+           apply IHn.
+           ++ unfold open_expr_wrt_expr. rewrite (size_expr_open_expr_wrt_expr_rec_var A1 x 0). lia.
+           ++ assumption.
+    + inversion H2. simpl in *. constructor.
+      * apply IHn. lia. assumption.
+      * intro. specialize (H6 x). apply lc_tobexpr. eapply IHn.
+        -- unfold open_expr_wrt_expr. rewrite (size_expr_open_expr_wrt_expr_rec_var B x 0). lia.
+        -- assumption.
+    + inversion H2. simpl in H1. constructor.
+      * constructor. apply IHn. lia. assumption.
+      * apply IHn. lia. assumption.
+    + inversion H1. simpl in H0. constructor.
+      * apply IHn. lia. assumption.
+(* P0 *)
+    + inversion H1. split; auto.
+Qed.        
+
+
+Theorem to_bcontext_keeps_lc : forall Γ, lc_context Γ -> lc_bcontext (to_bcontext Γ).
+Proof.
+  intros.
+  induction Γ.
+  - auto.
+  - simpl. constructor; inversion H; subst.
+    + apply IHΓ. auto.
+    + apply to_bexpr_keeps_lc. auto.
+Qed.
+
+
+Theorem to_bcontext_keeps_notin : forall x G, 
+  x `notin` ctx_dom G
+  -> x `notin` bctx_dom (to_bcontext G).
+Proof.
+  intros. induction G.
+  - auto.
+  - simpl in *.
+    specialize (notin_add_1' x0 x (ctx_dom G) H) as Hxx0.
+    specialize (notin_add_2 x0 x (ctx_dom G) H) as HxG.
+    apply notin_add_3; auto.
+Qed.
+
+Lemma wf_context_elab_keeps_lc : forall G Γ,
+    wf_context_elab Γ G
+    -> lc_context G
+    -> lc_bcontext Γ.
+Proof.
+  intros. induction H.
+  - constructor.
+  - constructor. inversion H0. auto.  
+Admitted.
+
+
+Check expr_ind.
+
 Lemma in_context_elab : forall Γ x A,
     x :_ A ∈ Γ -> ⊢ Γ -> forall Γ', wf_context_elab Γ' Γ -> exists A' k, in_bctx x A' Γ' /\ busub_elab Γ' A' A' d_infer ⧼k⧽' Γ A A ⧼(to_k k)⧽.
 Proof.
   intros * In Wf.
   induction In; intros.
   - inversion H1; subst. exists A', k.
-    split. eapply inb_here. admit. admit.
+    split. inversion H1. subst. eapply inb_here.
+    + inversion H6.  constructor. constructor.  admit.
+    + admit.
+    + admit.
+  - inversion H0. subst.
+    inversion Wf; subst.
+    specialize (IHIn H4 Γ'0 H5). destruct IHIn as [A'0 [k1 [IHInbctx  IHBusubElab]]].
+    exists A'0, k1. split. 
+    + apply inb_there. admit. auto.
+    + constructor. 
+    
+      admit. admit.
 Admitted.
 
-Theorem bidir_sound : forall Γ' e1' e2' d A' Γ e1 e2 A,
-  busub_elab Γ' e1' e2' d A' Γ e1 e2 A → Γ ⊢ e1 <: e2 : A.
-Proof.
-  intros.
-  induction H.
-  1-7: admit.
-  -
-    replace B with (B ^^ t) by admit.
-    eapply s_app.
-Admitted.
+Print usub_mut.
 
 Theorem bidir_complete : forall Γ e1 e2 A
   , Γ ⊢ e1 <: e2 : A
@@ -58,11 +250,49 @@ Proof.
   intros. pattern Γ, e1, e2, A, H.
   apply usub_mut with
     (P0 := fun Γ (_ : ⊢ Γ) => wf_context_elab (to_bcontext Γ) Γ); intros.
+  
+(* busub_elab *)
+  - constructor; auto. induction i; simpl in *.
+    + apply inb_here. apply to_bcontext_keeps_lc. auto. apply to_bexpr_keeps_lc. auto.
+    + apply inb_there. apply to_bexpr_keeps_lc. auto. 
+      eapply IHi. inversion w. auto. inversion H0. auto. 
+  - constructor. auto. 
+  - constructor. auto. 
+  - constructor. auto.
+  (* busub_elab *)
   - admit.
   - admit.
   - admit.
   - admit.
-  - simpl. eapply bse_anno.
+  - admit.
+  - admit.
+  - admit.
+  - admit.
+  - admit.
+  - admit.
+  - admit.
+    
+(* wf_context_elab *)
+  - constructor.
+  - simpl. apply (wfe_cons (to_bcontext G) G x (to_bexpr A0) A0 (to_bk k)).
+    + auto.
+    + apply to_bcontext_keeps_notin; auto.
+    + destruct k; auto.
+Admitted.
+
+
+Theorem bidir_sound : forall Γ' e1' e2' d A' Γ e1 e2 A,
+  busub_elab Γ' e1' e2' d A' Γ e1 e2 A → Γ ⊢ e1 <: e2 : A.
+Proof.
+  intros.
+  induct ion H.
+  (* pattern Γ', e1, e2', d, A', Γ, e1, e2, A, H.
+  eapply busub_ind_dep with 
+    (P0 := fun Γ' (_ : ⫦ Γ') => ⊢ Γ). *)
+  1-7: admit.
+  -
+    replace B with (B ^^ t) by admit.
+    eapply s_app.
 Admitted.
 
 
